Inserters/And.dfy
@@ -1,4 +1,4 @@
-module Build.SeqBuilder {
+module Inserters.And{
 
   import opened Circ
   import opened Eval
@@ -8,14 +8,27 @@ module Build.SeqBuilder {
   import opened ConservedSubcircuit
   import opened MapFunction
 
-  function SeqSF(si: SI): (so: SO)
-    requires |si.inputs| == 1
-    requires |si.state| == 1
+  function AndSF(si: SI): (so: SO)
+    requires |si.inputs| == 2
+    requires |si.state| == 0
   {
-    SO([si.state[0]], [si.inputs[0]])
+    SO([si.inputs[0] && si.inputs[1]], [])
   }
 
-  function InsertSeqImpl(c: Circuit): (r: (Circuit, Entity))
+  ghost predicate AndMFValid(mf: MapFunction)
+  {
+    && mf.Valid()
+    && |mf.inputs| == 2
+    && |mf.state| == 0
+    && |mf.outputs| == 1
+    && (forall si :: SIValid(si, mf.inputs, mf.state) ==> (
+      && mf.sf.requires(si)
+      && mf.sf(si) == AndSF(si)
+      )
+    )
+  }
+
+  function InsertAndImpl(c: Circuit): (r: (Circuit, Entity))
     requires CircuitValid(c)
     ensures CircuitValid(r.0)
     ensures EntitySomewhatValid(r.0, r.1)
@@ -25,15 +38,18 @@ module Build.SeqBuilder {
     var new_node := GetNewNode(c);
     assert new_node !in c.NodeKind;
     var new_c := Circuit(
-      NodeKind := c.NodeKind[new_node := CSeq],
+      NodeKind := c.NodeKind[new_node := CAnd],
       PortSource := c.PortSource
     );
     var i_0 := NP(new_node, INPUT_0);
+    var i_1 := NP(new_node, INPUT_1);
     var o_0 := NP(new_node, OUTPUT_0);
-    var inputs := [i_0];
+    var inputs := [i_0, i_1];
     var outputs := [o_0];
-    var state := [new_node];
-    var mf := MapFunction(inputs, outputs, state, SeqSF);
+    var state := [];
+    var mf := MapFunction(inputs, outputs, state, (si: SI) requires SIValid(si, inputs, state) =>
+      reveal Seq.ToSet();
+      SO([si.inputs[0] && si.inputs[1]], []));
     var e := Entity({new_node}, mf);
     assert EntitySomewhatValid(new_c, e) by {
       reveal EntitySomewhatValid();
@@ -55,18 +71,18 @@ module Build.SeqBuilder {
     (new_c, e)
   }
 
-  lemma InsertSeqCorrect(c: Circuit)
+  lemma InsertAndCorrect(c: Circuit)
     requires CircuitValid(c)
     ensures
-      var (new_c, e) := InsertSeqImpl(c);
+      var (new_c, e) := InsertAndImpl(c);
       && EntityValid(new_c, e)
   {
-    var (new_c, e) := InsertSeqImpl(c);
+    var (new_c, e) := InsertAndImpl(c);
     var o := e.mf.outputs[0];
     var i_0 := e.mf.inputs[0];
-    var os_0 := NP(e.mf.state[0], OUTPUT_0);
+    var i_1 := e.mf.inputs[1];
     var path := [e.mf.outputs[0]];
-    assert PathValid(new_c, path) && PathValid(new_c, [o, i_0]) by {
+    assert PathValid(new_c, path) && PathValid(new_c, [o, i_0]) && PathValid(new_c, [o, i_1]) by {
       reveal PathValid();
     }
     LengthOneNoDuplicates(path);
@@ -74,20 +90,26 @@ module Build.SeqBuilder {
     reveal Seq.ToSet();
     forall fi: FI | FIValid(fi, e.mf.inputs, e.mf.state)
       ensures
-        var sv_0 := fi.state[os_0.n];
+        var iv_0 := fi.inputs[i_0];
+        var iv_1 := fi.inputs[i_1];
         && FICircuitValid(new_c, fi)
-        && (EvaluateONP(new_c, o, fi) == EvalOk(sv_0))
+        && (EvaluateONP(new_c, o, fi) == EvalOk(iv_0 && iv_1))
     {
       var iv_0 := fi.inputs[i_0];
-      var sv_0 := fi.state[os_0.n];
+      var iv_1 := fi.inputs[i_1];
       assert Seq.HasNoDuplicates(path);
       assert FICircuitValid(new_c, fi) by {
         reveal MapFunction.Valid();
         reveal FICircuitValid();
       }
-      assert EvaluateONP(new_c, o, fi) == EvalOk(sv_0);
+      assert EvaluateONP(new_c, o, fi) == EvaluateONPBinary(new_c, [o], fi);
       reveal Seq.HasNoDuplicates();
-      assert Evaluate(new_c, o, fi) == EvalOk(sv_0);
+      assert EvaluateINPInner(new_c, [o, i_0], fi) == EvalOk(iv_0);
+      assert EvaluateINPInner(new_c, [o, i_1], fi) == EvalOk(iv_1);
+      assert EvaluateONPBinary(new_c, [o], fi) == EvalOk(iv_0 && iv_1);
+      assert EvaluateONPInner(new_c, [o], fi) == EvalOk(iv_0 && iv_1);
+      assert EvaluateONP(new_c, o, fi) == EvalOk(iv_0 && iv_1);
+      assert Evaluate(new_c, o, fi) == EvalOk(iv_0 && iv_1);
       assert Evaluate(new_c, o, fi) == EvalOk(e.mf.f(fi).outputs[o]) by {
         reveal MapMatchesSeqs();
       }
@@ -102,17 +124,17 @@ module Build.SeqBuilder {
     assert EntityValid(new_c, e);
   }
 
-  lemma InsertSeqConserves(c: Circuit)
+  lemma InsertAndConserves(c: Circuit)
     requires CircuitValid(c)
-    ensures CircuitConserved(c, InsertSeqImpl(c).0)
-    ensures CircuitUnconnected(c, InsertSeqImpl(c).0)
+    ensures CircuitConserved(c, InsertAndImpl(c).0)
+    ensures CircuitUnconnected(c, InsertAndImpl(c).0)
     ensures
-      var (new_c, e) := InsertSeqImpl(c);
+      var (new_c, e) := InsertAndImpl(c);
       IsIsland(new_c, e.sc)
   {
     reveal CircuitConserved();
     reveal CircuitUnconnected();
-    var (new_c, e) := InsertSeqImpl(c);
+    var (new_c, e) := InsertAndImpl(c);
     reveal CircuitValid();
     assert (forall np :: np in c.PortSource.Keys ==> np.n !in e.sc);
     assert (forall np :: np in c.PortSource.Values ==> np.n !in e.sc);
@@ -121,44 +143,20 @@ module Build.SeqBuilder {
     reveal IsIsland();
   }
 
-  lemma InsertSeqMFConsistent(c: Circuit)
+  function InsertAnd(c: Circuit): (r: (Circuit, Entity))
     requires CircuitValid(c)
     ensures
-      var (new_c, e) := InsertSeqImpl(c);
-      SeqRF().MFConsistent(e.mf)
+      var (new_c, e) := r;
+      && r == InsertAndImpl(c)
+      && CircuitValid(r.0)
+      && EntityValid(new_c, e)
+      && CircuitConserved(c, r.0)
+      && CircuitUnconnected(c, r.0)
+      && IsIsland(new_c, e.sc)
   {
-    reveal RFunction.MFConsistent();
-  }
-
-  function InsertSeq(c: Circuit): (r: (Circuit, Entity))
-    requires CircuitValid(c)
-    ensures SimpleInsertion(c, r.0, r.1)
-    ensures SeqRF().MFConsistent(r.1.mf)
-  {
-    InsertSeqCorrect(c);
-    InsertSeqConserves(c);
-    InsertSeqMFConsistent(c);
-    InsertSeqImpl(c)
-  }
-
-  const SeqRFConst := RFunction(1, 1, 1, SeqSF)
-
-  function SeqRF(): (r: RFunction)
-    ensures r.Valid()
-  {
-    reveal RFunction.Valid();
-    SeqRFConst
-  }
-
-  const SeqInserterConst := EntityInserter(SeqRF(), InsertSeq)
-
-  function SeqInserter(): (r: EntityInserter)
-    ensures r.Valid()
-  {
-    reveal RFunction.Valid();
-    reveal EntityInserter.Valid();
-    var rf := SeqRF();
-    SeqInserterConst
+    InsertAndCorrect(c);
+    InsertAndConserves(c);
+    InsertAndImpl(c)
   }
 
 }
