Modifiers/AppendReg.dfy
@@ -1,0 +1,71 @@
+module AppendReg {
+    
+  import opened Circ
+  import opened Entity
+  import opened Subcircuit
+  import opened ConservedSubcircuit
+  import opened IslandBundle
+  import opened Inserters.Reg
+  import opened CombineSeries
+  import opened MapFunction
+
+  function AppendRegSF(rf_base: RFunction, si: SI): (so: SO)
+    requires rf_base.Valid()
+    requires |si.inputs| == rf_base.input_width && |si.state| == rf_base.state_width + rf_base.output_width
+  {
+    var si_base := SI(si.inputs, si.state[..rf_base.state_width]);
+    reveal RFunction.Valid();
+    var so_base := rf_base.sf(si_base);
+    var old_reg_state := si.state[|si_base.state|..];
+    var so := SO(old_reg_state, so_base.state + so_base.outputs);
+    so
+  }
+
+  function AppendRegRF(rf_base: RFunction): (rf: RFunction)
+    requires rf_base.Valid()
+    ensures rf.Valid()
+  {
+    reveal RFunction.Valid();
+    RFunction(
+      rf_base.input_width,
+      rf_base.output_width,
+      rf_base.state_width + rf_base.output_width,
+      (si: SI) requires |si.inputs| == rf_base.input_width && |si.state| == rf_base.state_width + rf_base.output_width =>
+        AppendRegSF(rf_base, si)
+    )
+  }
+
+  lemma RFEquiv(rf_base: RFunction)
+    requires rf_base.Valid()
+    ensures
+      var reg_width := rf_base.output_width;
+      var rf_reg := RegRF(reg_width);
+      var rf_combined := CombineSeriesRF(rf_base, rf_reg);
+      var rf_appendreg := AppendRegRF(rf_base);
+      RFunctionEquiv(rf_appendreg, rf_combined)
+  {
+    reveal RFunction.Valid();
+    reveal RFunctionEquiv();
+  }
+
+  function AppendReg(c: Circuit, ei: EntityInserter): (r: (Circuit, Entity))
+    requires CircuitValid(c)
+    requires ei.Valid()
+    ensures SimpleInsertion(c, r.0, r.1)
+  {
+    var reg_width := ei.rf.output_width;
+    var ei_reg := RegInserter(reg_width);
+    var (c_a, e_a) := InsertTwoInSeries(c, ei, ei_reg);
+    reveal EntityInserter.Valid();
+    var new_rf := AppendRegRF(ei.rf);
+    RFEquiv(ei.rf);
+    var rf_combined := CombineSeriesRF(ei.rf, ei_reg.rf);
+    assert RFunctionEquiv(new_rf, rf_combined);
+    assert rf_combined.MFConsistent(e_a.mf);
+    MFConsistentEquiv(rf_combined, new_rf, e_a.mf);
+    assert new_rf.MFConsistent(e_a.mf);
+    var e_b := EntitySwapRF(c_a, e_a, new_rf);
+    (c_a, e_a)
+  }
+
+}
